total order on ms_hashfn_dom

Veritas.MultiSetHash.fsti
@@ -17,59 +17,60 @@ let ms_hash_value = bv_t ms_hash_size
 val empty_hash_value: ms_hash_value
 
 (* timestamp for blum *)
-type timestamp = 
+type timestamp =
   | MkTimestamp: e: nat -> c: nat -> timestamp
 
-let next (t: timestamp): timestamp = 
+let next (t: timestamp): timestamp =
   match t with
   | MkTimestamp e c -> MkTimestamp e (c + 1)
 
-let ts_lt (t1 t2: timestamp) = 
+let ts_lt (t1 t2: timestamp) =
   let e1 = MkTimestamp?.e t1 in
   let c1 = MkTimestamp?.c t1 in
   let e2 = MkTimestamp?.e t2 in
   let c2 = MkTimestamp?.c t2 in
   e1 < e2 || e1 = e2 && c1 < c2
 
-let ts_geq (t1 t2: timestamp) = 
+let ts_geq (t1 t2: timestamp) =
   not (ts_lt t1 t2)
 
-let ts_leq (t1 t2: timestamp) = 
+let ts_leq (t1 t2: timestamp) =
   t1 = t2 || t1 `ts_lt` t2
 
-let ts_gt (t1 t2: timestamp): bool = 
+let ts_gt (t1 t2: timestamp): bool =
   not (t1 `ts_leq` t2)
 
-type ms_hashfn_dom = 
+type ms_hashfn_dom =
   | MHDom: r:record -> t:timestamp -> i:nat -> ms_hashfn_dom
 
-let ms_hashfn_dom_cmp : cmp ms_hashfn_dom = magic ()
+val ms_hashfn_dom_cmp
+  : cmp ms_hashfn_dom
 
 type mset_ms_hashfn_dom = mset ms_hashfn_dom ms_hashfn_dom_cmp
 
-let key_of (e:ms_hashfn_dom): key = 
+let key_of (e:ms_hashfn_dom): key =
   match e with
   | MHDom (k,_) _ _ -> k
 
-let thread_id_of (e:ms_hashfn_dom): nat = 
+let thread_id_of (e:ms_hashfn_dom): nat =
   match e with
   | MHDom _ _ tid -> tid
 
 let is_of_thread_id (tid:nat) (e:ms_hashfn_dom): bool =
   thread_id_of e = tid
 
-let timestamp_of (e:ms_hashfn_dom): timestamp = 
+let timestamp_of (e:ms_hashfn_dom): timestamp =
   match e with
   | MHDom _ t _ -> t
 
-(* 
- * incremental multiset hash function - update the 
+(*
+ * incremental multiset hash function - update the
  * hash given a new element
  *)
 val ms_hashfn_upd (e: ms_hashfn_dom) (h: ms_hash_value): Tot ms_hash_value
 
 (* multiset hash function for a sequence *)
-val ms_hashfn (s: seq ms_hashfn_dom): Tot ms_hash_value 
+val ms_hashfn (s: seq ms_hashfn_dom): Tot ms_hash_value
 
 (* two sequences that encode the same multiset produce the same hash *)
 val lemma_mshashfn_correct (s1 s2: seq ms_hashfn_dom):
@@ -91,8 +92,8 @@ val lemma_hashfn_agg (s1 s2: seq ms_hashfn_dom):
   Lemma (ms_hashfn (append s1 s2) = ms_hashfn_agg (ms_hashfn s1) (ms_hashfn s2))
 
 (* multiset hash collision *)
-type ms_hash_collision = 
-  | MSCollision: s1: seq ms_hashfn_dom -> 
+type ms_hash_collision =
+  | MSCollision: s1: seq ms_hashfn_dom ->
                  s2: seq ms_hashfn_dom { ms_hashfn s1 = ms_hashfn s2 /\
                                          ~(seq2mset #_ #ms_hashfn_dom_cmp s1 ==
                                            seq2mset #_ #ms_hashfn_dom_cmp s2)} -> ms_hash_collision
